Source/DafnyRuntime/DafnyRuntimeDafny/src/dafnyRuntime.dfy
@@ -468,6 +468,29 @@ abstract module {:options "/functionSyntax:4"} Dafny {
       this
     }
 
+    // The following function signature is a LIE. It says that it will return a set<X>
+    // for any given X and any f, but it does it only if T and X are the same type
+    // and f is the identity function. Stated differently, the function return the set
+    // of elements in Sequence<T>, but it can do so only if T is an equality-supporting
+    // type.
+    //
+    // Dafny does support the UniqueElements operation (for example, when a "forall"
+    // statement needs it), but will make use of it only if T is an equality-supporting
+    // type. The proper way to express that in Dafny is to declare a method outside the
+    // class:
+    //
+    //     function {:extern} UniqueElements<X(==)>(s: Sequence<X>): set<X>
+    //       requires s.Valid()
+    //       ensures UniqueElements(s) == set t | t in s.Value()
+    //
+    // However, because the Go implementation (and perhaps the implementation of other
+    // targets, too) relies on the method being an instance method, there's a mismatch.
+    // Thus, for now, the best way to proceed seems to be to include the additional type
+    // parameter X here.
+    function {:extern} UniqueElements<X(==)>(ghost f: T -> X): set<X>
+      requires Valid() /* AND X==T AND f is the identity function, see above */
+      ensures UniqueElements(f) == set t | t in Value() :: f(t)
+
     // Sequence creation methods
 
     static method Create<T>(cardinality: size_t, initFn: size_t -> T) returns (ret: Sequence<T>) {
